# 23 - Converting to CNF via NNF

See `moreCNFSentences`.
You will find the following sentences in every third position.

- ¬[(Sqr(a) ∧ ¬Sml(a)) ∧ (¬Sqr(a) ∨ Sml(a))]
- ¬((Sqr(a) ∨ ¬Sml(a)) ∧ (¬Sqr(a) ∨ Sml(a)))

- The two blanks that follow each sentence are for you to:
  - first transform the sentence into negation normal form (NNF),
  - and then put that NNF sentence into conjunctive normal form (CNF).
- Again, check your work by opening several worlds to see
  that each of your sentences has the same truth value as the original.
- When you are finished, save the modified sentences.
